[Scheme] opt CPS rich semantics

compiler/scheme/cps/optCpsScript.sml
@@ -11,6 +11,18 @@ Datatype:
   richcbvctxt = RCFn cbvexp | RCArg 'a
 End
 
+Datatype:
+  valtag = TVar string | TAbs
+End
+
+Datatype:
+  richcbvstate = RCExp cbvexp | RCVal bool valtag cbvval
+End
+
+Datatype:
+  valtype = Trivial valtag | Computation
+End
+
 Definition count_rcarg_def:
   count_rcarg [] = 0 /\
   count_rcarg (RCFn _::ks) = count_rcarg ks /\
@@ -36,3 +48,67 @@ Definition opt_cps_def:
 Termination
   cheat
 End
+
+Definition rich_cbv_continue_def:
+  rich_cbv_continue [] env scopes comp tag v = (case scopes of
+  | [] => ([], env, [], RCVal comp tag v)
+  | (env', ks)::scopes' => (ks, env', scopes', RCVal T tag v)) /\
+  rich_cbv_continue (RCFn e::ks) env scopes comp tag v = (if comp
+    then ((RCArg (Computation, v)::ks), env, scopes, RCExp e)
+    else ((RCArg (Trivial tag, v)::ks), env, scopes, RCExp e)) /\
+  rich_cbv_continue (RCArg (vtype, vfn)::ks) env scopes comp tag v = (case vfn of
+  | VCl x env' e => ([], nsBind x v env', (env, ks)::scopes, RCExp e))
+End
+
+Definition rich_cbv_step_def:
+  rich_cbv_step (ks, env, scopes, RCVal comp tag v) = rich_cbv_continue ks env scopes comp tag v /\
+  rich_cbv_step (ks, env, scopes, RCExp (EVar x)) = (ks, env, scopes, RCVal F (TVar x) (strict_lookup env x)) /\
+  rich_cbv_step (ks, env, scopes, RCExp (EAbs x e)) = (ks, env, scopes, RCVal F TAbs (VCl x env e)) /\
+  rich_cbv_step (ks, env, scopes, RCExp (EApp e1 e2)) = (RCFn e2::ks, env, scopes, RCExp e1)
+End
+
+Definition ctxt_with_env_def:
+  ctxt_with_env env (RCFn e) = CFn env e /\
+  ctxt_with_env env (RCArg (vtype, v)) = CArg v
+End
+
+Definition cat_ks_def:
+  cat_ks ks env scopes = FLAT (MAP (\(env, ks). MAP (ctxt_with_env env) ks) ((env, ks)::scopes))
+End
+
+Definition forget_def:
+  forget (ks, env, scopes, RCVal comp tag v) = (cat_ks ks env scopes, CVal v) /\
+  forget (ks, env, scopes, RCExp e) = (cat_ks ks env scopes, CExp env e)
+End
+
+Theorem forget_rich:
+  ! ks ks' env env' scopes scopes' e e' .
+    rich_cbv_step (ks, env, scopes, e) = (ks', env', scopes', e')
+    ==>
+    cbv_step (forget (ks, env, scopes, e)) = forget (ks', env', scopes', e') \/
+    forget (ks, env, scopes, e) = forget (ks', env', scopes', e')
+Proof
+  rpt strip_tac
+  >> Cases_on `e`
+  >~ [`RCExp e`] >>> HEADGOAL $ Cases_on `e`
+  >~ [`RCVal comp tag v`]
+  >>> HEADGOAL (
+    Cases_on `ks`
+    >~ [`k::ks'`]
+    >>> HEADGOAL (
+      Cases_on `k`
+      >~ [`RCFn e`] >>> HEADGOAL $ Cases_on `comp`
+      >~ [`RCArg tagv`]
+      >>> HEADGOAL (
+        PairCases_on `tagv`
+        >> Cases_on `tagv1`
+      )
+    )
+    >>> LASTGOAL (
+      Cases_on `scopes`
+      >~ [`scope::scopes'`]
+      >>> HEADGOAL $ PairCases_on `scope`
+    )
+  )
+  >> gvs[forget_def, rich_cbv_step_def, rich_cbv_continue_def, cbv_step_def, cbv_continue_def, cat_ks_def, ctxt_with_env_def]
+QED
